all pure functions now translate

translator/ml_translatorLib.sml
@@ -1546,6 +1546,16 @@ fun rm_fix res = let
   val tm2 = QCONV (REWRITE_CONV [lemma]) res |> concl |> dest_eq |> snd
   in tm2 end
 
+val MAP_pattern = ``MAP (f:'a->'b)``
+
+(*
+val tm = rhs
+
+val tm = ``MAP (\v3. type_subst v6 v3) args``
+val tm = ``MAP (\v3. type_subst v6 v3)``
+
+*)
+
 fun hol2deep tm =
   (* variables *)
   if is_var tm then let
@@ -1605,7 +1615,7 @@ fun hol2deep tm =
     val (p,x1,x2,lemma) = dest_builtin_binop tm
     val th1 = hol2deep x1
     val th2 = hol2deep x2
-    val result = MATCH_MP (MATCH_MP lemma th1) th2 |> UNDISCH_ALL
+    val result = MATCH_MP (MATCH_MP lemma th1) (UNDISCH_ALL th2) |> UNDISCH_ALL
     in check_inv "binop" tm result end else
   (* boolean not *)
   if can (match_term ``~(b:bool)``) tm then let
@@ -1653,6 +1663,28 @@ fun hol2deep tm =
     val th2 = INST [v|->z] th2
     val result = MATCH_MP Eval_Let (CONJ th1 th2)
     in check_inv "let" tm result end else
+  (* special pattern *) let
+    val _ = match_term MAP_pattern tm
+    val (m,f) = dest_comb tm
+    val th_m = hol2deep ``MAP:('a->'b) -> 'a list -> 'b list``
+    val (v,x) = dest_abs f
+    val th_f = hol2deep x
+    val th_f = apply_Eval_Fun v th_f true
+    val thi = th_f |> DISCH_ALL |> RW [AND_IMP_INTRO] |> GEN v
+    val thi = HO_MATCH_MP Eq_IMP_And thi
+    val thi = MATCH_MP (MATCH_MP Eval_Arrow th_m) thi
+    val list_type_def = fetch "-" "LIST_TYPE_def"
+    val LIST_TYPE_And = prove(
+     ``LIST_TYPE (And a P) = And (LIST_TYPE a) (EVERY (P:'a->bool))``,
+     SIMP_TAC std_ss [FUN_EQ_THM,And_def] \\ Induct
+     \\ FULL_SIMP_TAC std_ss [MEM,list_type_def]
+     \\ REPEAT STRIP_TAC \\ EQ_TAC \\ REPEAT STRIP_TAC
+     \\ FULL_SIMP_TAC (srw_ss()) [And_def])
+    val thi = RW [LIST_TYPE_And] thi
+    val thi = MATCH_MP And_IMP_Eq thi |> SIMP_RULE std_ss [EVERY_MEM]
+    val thi = thi |> CONV_RULE ((RATOR_CONV o RAND_CONV) (REWR_CONV (GSYM PRECONDITION_def)))
+    val result = thi |> UNDISCH_ALL
+    in check_inv "map" tm result end handle HOL_ERR _ =>
   (* normal function applications *)
   if is_comb tm then let
     val (f,x) = dest_comb tm
@@ -1897,6 +1929,7 @@ fun translate def = let
       \\ FULL_SIMP_TAC (srw_ss()) [ADD1]
       \\ REPEAT STRIP_TAC
       \\ FULL_SIMP_TAC (srw_ss()) [ADD1]
+      \\ FULL_SIMP_TAC std_ss [pair_case_def]
       \\ METIS_TAC []);
     val th = UNDISCH lemma |> SPECL (rev rev_params)
     val th = RW [PreImp_def] th |> UNDISCH_ALL
